Todo: clean

LazyReduction/WordByWordMontgomeryLazyReduction.v
@@ -49,7 +49,7 @@ Module WordByWordMontgomery.
          v ++ [c].
     Let SOS_red_add {n n'} (p : T n) ( q : T n') :  T (n)
         := let '(v,c) := (Rows.add weight n p (Positional.extend_to_length n' n q)) in
-    v.
+         v.
     Let drop_high_addT' {n} (p : T (S n)) (q : T n) : T (S n) (* drops carry *)
       := fst (Rows.add weight (S n) p (Positional.extend_to_length n (S n) q)).
     Let conditional_sub {n} (arg : T (S n)) (N : T n) : T n  (* computes [arg - N] if [N <= arg], and drops high bit *)
@@ -58,6 +58,8 @@ Module WordByWordMontgomery.
             (N : T R_numlimbs). (* encoding of m *)
     Let sub_then_maybe_add (a b : T R_numlimbs) : T R_numlimbs (* computes [a - b + if (a - b) <? 0 then N else 0] *)
       := fst (Rows.sub_then_maybe_add weight R_numlimbs (r-1) a b N).
+      Let T_app {n} (p : T n) (e : Z) : T (S n)
+      := p ++ [e].
     Local Opaque T.
     Section red_iteration.
     Context (pred_A_numlimbs : nat)
@@ -83,6 +85,8 @@ Module WordByWordMontgomery.
         S2.
 
         Check red_steps.
+        Check A.
+        Check SOS_red_add.
     Lemma red_steps': red_steps = S2. Proof. reflexivity. Qed.
         
     End red_iteration.
@@ -108,8 +112,12 @@ Module WordByWordMontgomery.
   => red_loop_count' (red_body A))
   count.
   Definition pre_red : T (2 * N_numlimbs + 1)
-  := dlet res := (red_loop num_it (Positional.extend_to_length (2 * N_numlimbs) (2 * N_numlimbs + 1) A)) in
-    res.
+  := (red_loop num_it (Positional.extend_to_length (2 * N_numlimbs) (2 * N_numlimbs + 1) A)).
+
+    Definition red : T (R_numlimbs )
+    := dlet res
+      := conditional_sub (red_loop R_numlimbs (Positional.extend_to_length (2 * R_numlimbs) (2 * R_numlimbs + 1) A)) N in
+      res.
 End red_loop. 
 
 
@@ -129,6 +137,8 @@ End red_loop.
     Transparent T.
     Definition small {n} (v : T n) : Prop
       := v = Partition.partition weight n (eval v).
+    Definition sc_small sc : Prop
+      := 0 <= sc < r.  
     Context (small_N : small N)
             (N_lt_R : eval N < R)
             (N_nz : 0 < eval N)
@@ -136,7 +146,8 @@ End red_loop.
             (B_bounds : 0 <= eval B < R)
             (small_B : small B)
             ri (ri_correct : r*ri mod (eval N) = 1 mod (eval N))
-            (k : Z) (k_correct : k * eval N mod r = (-1) mod r).
+            (k : Z) (k_correct : k * eval N mod r = (-1) mod r)
+            (numbits_big: Z.of_nat R_numlimbs < r).
 
     Local Lemma r_big : r > 1.
     Proof using lgr_big. clear -lgr_big; subst r. auto with zarith. Qed.
@@ -216,6 +227,36 @@ End red_loop.
         all: nia. }
     Qed.
 
+    Definition app_hyp v1 : list Z -> Prop
+    := fun v2 => 
+        (
+          @eval (length v1 + length v2) (v1 ++ v2) = @eval (length v1) v1 + r ^ Z.of_nat (length v1) * @eval (length v2) v2
+        ).
+
+        Lemma eval_sc: forall sc, @eval 1 [sc] = sc.
+    Proof.
+      intros. unfold eval, Positional.eval, Associational.eval, Positional.to_associational.
+      simpl. rewrite weight_0; [auto with zarith | apply wprops].
+    Qed. 
+
+    Lemma eval_app: forall (n1 n2 : nat) v1 v2, length v1 = n1 -> length v2 = n2 -> @eval (n1 + n2) (v1 ++ v2) = @eval n1 v1 + (r ^ (Z.of_nat (length v1)) * (@eval n2 v2)).
+    Proof.
+      intros. generalize dependent n1. generalize dependent n2.
+      pose proof (@rev_ind Z (app_hyp v1)). unfold app_hyp in H. intros. unfold eval.
+      rewrite <- H1. rewrite <- H0. apply H.
+        - unfold eval. rewrite Positional.eval_nil. rewrite Z.mul_0_r. simpl.
+          repeat rewrite Z.add_0_r. Local Close Scope Z_scope. assert (length v1 + 0 = length v1) by auto.
+          rewrite H2. rewrite app_nil_r. auto.
+        - intros. unfold eval. rewrite app_length. simpl. Search (_ + 1). rewrite Nat.add_1_r.
+          assert (v1 ++ l ++ [x] = (v1 ++ l) ++ [x]) by apply app_assoc. rewrite H3.
+          Search (_ + S _). rewrite NPeano.Nat.add_succ_r.
+          rewrite Positional.eval_snoc_S. rewrite Positional.eval_snoc_S.
+          simpl. unfold eval in H2. rewrite H2. simpl.
+          rewrite Z.mul_add_distr_l. rewrite Z.mul_assoc. About Weight. rewrite uweight_sum_indices.
+          rewrite uweight_eq_alt. unfold r. auto with zarith.
+          all: try rewrite app_length; auto with zarith. Local Open Scope Z_scope.
+    Qed.
+
     Local Ltac push_step :=
       first [ progress eta_expand
             | rewrite Rows.mul_partitions
@@ -254,6 +295,7 @@ End red_loop.
     Qed.
     Local Hint Immediate small_zero : core.
 
+
     Ltac push_recursive_partition :=
       repeat match goal with
              | _ => progress cbn [recursive_partition]
@@ -289,6 +331,7 @@ End red_loop.
       push_recursive_partition; cbn [Rows.divmod snd hd].
       autorewrite with zsimplify; reflexivity.
     Qed.
+
     Lemma small_div : forall n v, small v -> small (fst (@divmod n v)).
     Proof using lgr_big.
       pose proof r_big as r_big.
@@ -318,6 +361,116 @@ End red_loop.
       rewrite Hv. autorewrite with push_eval.
       apply partition_eq_mod; auto; [ ].
       Z.rewrite_mod_small; reflexivity.
+    Qed.
+
+
+    Lemma small_nil: @small 0 [].
+    Proof. reflexivity. Qed.
+    
+    Definition small_crit n v := (Forall sc_small v) /\ (length v = n).
+
+    Lemma length_S_app: forall (l: list Z) n, length l = S n -> exists l' a, l = @T_app (n) l' a.
+    Proof. intros l. apply (rev_ind (fun (y : list Z) => (forall n, length y = S (n) -> exists l' a, y = l' ++ [a]))).
+      - intros. discriminate.
+      - intros. exists l0, x. auto.
+    Qed.
+
+    Lemma weight_value: forall n, weight n = r ^ (Z.of_nat n).
+    Proof.
+      intros; rewrite uweight_eq_alt'; apply Z.pow_mul_r; lia.
+    Qed.
+
+    Lemma r_pow_S : forall n, r ^ (Z.of_nat (S n)) = r ^ (Z.of_nat n) * r.
+    Proof.
+      intros; rewrite Nat2Z.inj_succ; rewrite Z.pow_succ_r; auto with zarith.
+    Qed.
+
+    Lemma sc_small_length_small: forall n (v: T n), length v = n -> Forall sc_small v -> small v.
+    Proof. intros. generalize dependent v. induction n.
+        - intros. rewrite length_zero_iff_nil in H. rewrite H. apply small_nil.
+        - intros. assert (H': length v = S n) by auto. apply length_S_app in H. destruct H, H.
+          assert (small x).
+            + apply IHn. apply (f_equal (fun (y : list Z) => length y)) in H. unfold T_app in H.
+              rewrite app_length in H. rewrite H' in H. simpl in H. rewrite Nat.add_1_r in H. inversion H.
+              auto.
+              unfold T_app in H. rewrite H in H0. rewrite Forall_app in H0. destruct H0. auto.
+            + unfold T_app in H. rewrite H. unfold small. rewrite Partition.partition_step.
+              rewrite H in H'. rewrite app_length in H'. simpl in H'.
+              rewrite Nat.add_1_r in H'. inversion H'.
+              assert (Partition.partition weight n (@eval (S n) (x ++ [x0])) = Partition.partition weight n (@eval n (x))).
+                { apply Partition.partition_eq_mod; auto. rewrite <- Nat.add_1_r.
+                  rewrite eval_app; auto. rewrite H3.
+                   rewrite weight_value. rewrite Z.mod_add'_full. auto. }
+              assert (@eval (S n) (x ++ [x0]) mod weight (S n) / weight n = x0).
+              {
+                rewrite <- Nat.add_1_r. rewrite eval_app; auto.
+                Search ( (_ + _) / _ ). rewrite uweight_pull_mod; auto with zarith.
+                assert (n + 1 - n = 1)%nat by auto with zarith. rewrite H4.
+                rewrite (weight_value n). rewrite H3. rewrite Z.div_add'.
+                Search (_ / _ = 0). rewrite Zdiv_small.
+                  - rewrite eval_sc. simpl. apply Z.mod_small.
+                    assert (sc_small x0).
+                      + apply (Forall_forall sc_small v); auto. rewrite H. Search (In (_ ++ _)).
+                        apply in_or_app. right. simpl. auto.
+                      + unfold sc_small in H5. rewrite weight_value. auto with zarith.
+                  - apply small_bound in H1. rewrite weight_value in H1. auto.
+                  - unfold r; auto with zarith.
+              }
+              unfold small in H1. rewrite H3, H2, H4. rewrite <- H1. auto.
+    Qed.
+
+    Lemma small_rem: forall n (v : T n) x, @small (S n) (v ++ [x]) -> small v.
+    Proof.
+      intros. pose proof (length_small H). rewrite app_length in H0. rewrite Nat.add_1_r in H0. inversion H0.
+      unfold small in H. rewrite Partition.partition_step in H. rewrite <- Nat.add_1_r in H. rewrite eval_app in H; auto.
+      Search ((_ ++ [_]) = (_ ++ [_])). apply app_inj_tail in H. destruct H.
+      unfold small.
+      assert ( Partition.partition weight n
+      (eval v + r ^ Z.of_nat (length v) * @eval 1 [x]) = Partition.partition weight (length v) (eval v)).
+        - rewrite H2. apply Partition.partition_eq_mod; auto.
+          rewrite weight_value. rewrite Z.mod_add'_full. auto.
+        - rewrite H2. rewrite H2 in H3. rewrite <- H3. auto. rewrite H2 in H. auto.
+    Qed.
+
+    Lemma small_sc_small: forall n (v : T n), small v -> Forall sc_small v.
+    Proof. intros.
+      apply (rev_ind (fun v => (@small (length v) v -> Forall sc_small v))); auto.
+      intros. rewrite Forall_app; split.
+        - apply H0. Set Printing All. apply (small_rem) with (x := x). auto. simpl in H1.
+          unfold small in H1. unfold small. rewrite app_length in H1. simpl in H1. rewrite Nat.add_1_r in H1. auto.
+        - apply Forall_cons; auto. unfold small in H1.
+          rewrite app_length in H1. simpl in H1. rewrite Nat.add_1_r in H1. rewrite Partition.partition_step in H1.
+          apply app_inj_tail in H1. destruct H1. rewrite uweight_pull_mod in H2; auto; try lia.
+          assert (forall n, (S n - n = 1)% nat). auto with zarith. rewrite H3 in H2. rewrite weight_value in H2.
+          Search ((_ mod _) < _). unfold sc_small. rewrite H2. rewrite weight_value.
+          assert (r ^ Z.of_nat 1 = r). auto with zarith. rewrite H4. apply Z.mod_pos_bound. unfold r. auto with zarith.
+        - pose proof (length_small H). rewrite H0. auto.
+    Qed.
+
+    Lemma small_if_Forall_sc_small: forall n (v : T n),
+    small v <-> (length v = n) /\ (Forall sc_small v).
+    Proof.
+      repeat split; intros; [apply length_small; auto| apply small_sc_small; auto| apply sc_small_length_small; destruct H; auto].
+    Qed.
+    
+    Lemma small_s_mod: forall n (A : T (S n)), small A -> with_args.s n A = eval A mod r.
+    Proof.
+      intros. unfold s. simpl. apply small_if_Forall_sc_small in H. destruct H.
+      destruct A.
+        - simpl. unfold eval. rewrite Positional.eval_nil. auto.
+        - simpl. Search (Forall _ (_ :: _)). apply Forall_inv in H0. unfold sc_small in H0.
+          assert (z :: A = ([z] ++ A)). auto.
+          rewrite H1. pose proof (eval_app 1 n [z] A).
+          Set Printing All. assert ((Init.Nat.add (S O) n) = (S n)). auto.
+          Set Printing All.
+          rewrite H3 in H2.
+          rewrite H2.
+          simpl. Search (Z.pow_pos _ 1). rewrite Zpow_facts.Zpower_pos_1_r.
+          rewrite Z.mod_add'.
+          rewrite Z.mod_small. rewrite eval_sc; auto. rewrite eval_sc; auto.
+          auto with zarith.
+          auto.
+          auto.
     Qed.
 
     Local Lemma scmul_correct: forall n a v, small v -> 0 <= a < r -> 0 <= eval v < r^Z.of_nat n -> canon_rep (a * eval v) (@scmul n a v).
@@ -409,30 +562,6 @@ End red_loop.
     Qed.
     Check Positional.zeros.
 
-    Definition app_hyp v1 : list Z -> Prop
-    := fun v2 => 
-        (
-          @eval (length v1 + length v2) (v1 ++ v2) = @eval (length v1) v1 + r ^ Z.of_nat (length v1) * @eval (length v2) v2
-        ).
-
-    Lemma eval_app: forall (n1 n2 : nat) v1 v2, length v1 = n1 -> length v2 = n2 -> @eval (n1 + n2) (v1 ++ v2) = @eval n1 v1 + (r ^ (Z.of_nat (length v1)) * (@eval n2 v2)).
-    Proof.
-      intros. generalize dependent n1. generalize dependent n2.
-      pose proof (@rev_ind Z (app_hyp v1)). unfold app_hyp in H. intros. unfold eval.
-      rewrite <- H1. rewrite <- H0. apply H.
-        - unfold eval. rewrite Positional.eval_nil. rewrite Z.mul_0_r. simpl.
-          repeat rewrite Z.add_0_r. Local Close Scope Z_scope. assert (length v1 + 0 = length v1) by auto.
-          rewrite H2. rewrite app_nil_r. auto.
-        - intros. unfold eval. rewrite app_length. simpl. Search (_ + 1). rewrite Nat.add_1_r.
-          assert (v1 ++ l ++ [x] = (v1 ++ l) ++ [x]) by apply app_assoc. rewrite H3.
-          Search (_ + S _). rewrite NPeano.Nat.add_succ_r.
-          rewrite Positional.eval_snoc_S. rewrite Positional.eval_snoc_S.
-          simpl. unfold eval in H2. rewrite H2. simpl.
-          rewrite Z.mul_add_distr_l. rewrite Z.mul_assoc. About Weight. rewrite uweight_sum_indices.
-          rewrite uweight_eq_alt. unfold r. auto with zarith.
-          all: try rewrite app_length; auto with zarith.
-    Qed.
-
     Lemma nat_sub: forall x y, (S x <= y)%nat -> S (y - S x) = (y - x)%nat.
     Proof.
        intros. rewrite <- Nat.sub_succ_l. rewrite NPeano.Nat.sub_succ; auto. auto. Qed.
@@ -447,6 +576,12 @@ End red_loop.
     Proof.
       intros. unfold Positional.extend_to_length. assert ((n1 + n2 - n1)%nat = n2) by auto with zarith.
       rewrite H. auto.
+    Qed.
+
+    Lemma extend_length: forall n1 n2 v, (length v = n2)%nat -> (n2 <= n1)%nat -> length (Positional.extend_to_length n2 n1 v) = n1.
+    Proof.
+      intros. assert (n1 = n2 + (n1 - n2))%nat by auto with zarith. rewrite H1. rewrite extend_app.
+      rewrite app_length. rewrite Positional.length_zeros. auto.
     Qed.
 
     Lemma zeros_S: forall n, Positional.zeros (S n) = (Positional.zeros n ++ [0%Z]).
@@ -467,6 +602,7 @@ End red_loop.
           + lia.
     Qed.
 
+    Local Close Scope Z_scope.
     Lemma weight_geq': forall n1 n2, n2 <= n1 -> ((weight n2) <= (weight n1))%Z.
     Proof.
       intros. assert ((n1 = (n2 + (n1 - n2)))). auto with zarith. rewrite H0.
@@ -491,10 +627,9 @@ End red_loop.
     Proof. intros. destruct A; [contradiction| auto]. Qed.
 
 
-
-    Lemma small_exten: forall n1 n2 (v : T n2), (n2 <= n1)%nat -> small v -> @small n1 (Positional.extend_to_length n2 n1 v).
+    Lemma small_exten: forall n1 (n2: nat) (v : T n2), (n2 <= n1)%nat -> small v -> @small n1 (Positional.extend_to_length n2 n1 v).
     Proof. intros. Search small. apply small_canon_rep with (x := (eval v)). split.
-      - assert (n1 = n2 + (n1 - n2)) by auto with zarith. rewrite H1. rewrite Partition_long.
+      - assert ((n1 = n2 + (n1 - n2))%nat) by auto with zarith. rewrite H1. rewrite Partition_long.
         simpl. rewrite <- H1. reflexivity. auto.
       - pose proof (small_bound H0). pose proof (weight_geq' n1 n2). lia.
     Qed.
@@ -521,20 +656,141 @@ End red_loop.
     Proof using small_N lgr_big R_numlimbs_nz N_nz N_lt_R. eauto using sub_then_maybe_add_correct, eval_canon_rep. Qed.
     Local Lemma small_sub_then_maybe_add : forall a b, small a -> small b -> 0 <= eval a < eval N -> 0 <= eval b < eval N -> small (sub_then_maybe_add a b).
     Proof using small_N lgr_big R_numlimbs_nz N_nz N_lt_R. eauto using sub_then_maybe_add_correct, small_canon_rep. Qed.
+          
 
-    Lemma small_nil: @small 0 [].
-    Proof.
-      unfold small, Partition.partition. simpl. auto.
+    Lemma eval_extend: forall n1 n2 (v : T n2), (n2 <= n1)%nat -> length v = n2 -> eval v =  @eval n1 (Positional.extend_to_length n2 n1 v).
+    Proof. intros. assert (n1 = n2 + (n1 - n2))%nat by auto with zarith. rewrite H1. rewrite extend_app.
+      rewrite eval_app; try rewrite Positional.length_zeros; auto. rewrite eval_zero. auto with zarith.
     Qed.
 
     Lemma small_SOS_red_add: forall n1 n2 (v1 : T n1) (v2 : T n2), (n2 <= n1)%nat -> small v1 -> small v2 -> small (SOS_red_add v1 v2).
+    Proof. intros.
+      destruct n1 eqn:eq1.
+        - assert (n2 = 0)%nat by auto with zarith. apply length_small in H0. apply length_small in H1.
+          rewrite H2 in H1. Search (length _ = O). apply length_zero_iff_nil in H0.
+          apply length_zero_iff_nil in H1. rewrite H0, H1.
+          unfold SOS_red_add. simpl. apply small_nil.
+         - intros. unfold SOS_red_add. assert (@small n1 (Positional.extend_to_length n2 n1 v2)) by (apply small_exten; auto; lia).
+          rewrite eq1 in H2.
+          pose proof (small_addT (S n) v1 (Positional.extend_to_length n2 (S n) v2) H0 H2). unfold addT in H3.
+          remember ( Rows.add weight (S n) v1 (Positional.extend_to_length n2 (S n) v2)) as v'.
+          destruct v'. apply small_rem with (x := z). auto.
+    Qed.
+    
+
+    Lemma eval_SOS_red_add_mod: forall n1 n2 (v1 : T n1) (v2 : T n2), (n2 <= n1)%nat -> small v1 -> small v2 -> eval (SOS_red_add v1 v2) = (eval v1 + eval v2) mod r ^ Z.of_nat n1.
     Proof.
-    Admitted.
+      intros. unfold SOS_red_add. simpl. unfold eval. rewrite Rows.sum_rows_mod; auto.
+        - rewrite weight_value. rewrite <- eval_extend with (n1 := n1); try apply length_small; auto.
+        - apply length_small; auto.
+        - rewrite extend_length; try apply length_small; auto.
+    Qed.
+
+    Lemma eval_SOS_add_full: forall n1 n2 (v1 : T n1) (v2 : T n2), (n2 <= n1)%nat -> small v1 -> small v2 ->
+      eval (SOS_red_add v1 v2) + (weight n1 * ((eval v1 + eval v2) / weight n1)) = (eval v1 + eval v2).
+    Proof.
+      intros. unfold SOS_red_add. simpl. unfold eval. rewrite Rows.sum_rows_mod; try apply extend_length; try apply length_small; auto.
+      rewrite <- eval_extend with (n1 := n1); try apply length_small; auto.  rewrite <- Z.div_mod''; auto.
+    Qed.
+
+    Lemma eval_SOS_add_full': forall n1 n2 (v1 : T n1) (v2 : T n2), (n2 <= n1)%nat -> small v1 -> small v2 ->
+    eval (SOS_red_add v1 v2) = (eval v1 + eval v2) - (weight n1 * ((eval v1 + eval v2) / weight n1)).
+  Proof.
+    intros. pose proof (eval_SOS_add_full n1 n2 v1 v2 H H0 H1). apply (f_equal (fun y => y - (weight n1 * ((eval v1 + eval v2) / weight n1)))) in H2.
+    assert (forall (x : Z) y, x + y - y = x). auto with zarith. rewrite H3 in H2. auto.
+  Qed.
+
+  Lemma eval_SOS_add_small: forall n1 n2 (v1 : T n1) (v2 : T n2), (n2 <= n1)%nat -> small v1 -> small v2 ->
+    (eval v1 + eval v2) < (weight n1)  -> eval (SOS_red_add v1 v2) = (eval v1 + eval v2).
+  Proof.
+    intros. rewrite eval_SOS_add_full'; auto. rewrite Zdiv_small; auto with zarith.
+    apply small_bound in H0. apply small_bound in H1. lia.
+  Qed.
+
+  Lemma eval_SOS_bound: forall n1 n2 (v1 : T n1) (v2 : T n2), (n2 <= n1)%nat -> small v1 -> small v2 ->
+    eval (SOS_red_add v1 v2) <= eval v1 + eval v2.
+  Proof.
+    intros. rewrite <- eval_SOS_add_full; auto with zarith. Search (?n1 <= ?n1 + _).
+    pose proof (@small_bound _ v1 H0). pose proof (@small_bound _ v2 H1).
+    assert (0 <= eval v1 + eval v2) by lia. assert (0 <= (eval v1 + eval v2) / weight n1 ). apply Z.div_nonneg.
+     lia. lia. assert (0 <= weight n1 * ((eval v1 + eval v2) / weight n1)). Search (0 <= _ * _).
+     apply Z.mul_nonneg_nonneg; lia. lia.
+  Qed.
+
+  Lemma smallthism': forall n (A : T (S n)), sc_small (thism n A k).
+  Proof. intros. unfold thism; rewrite Z.mul_split_mod; unfold sc_small; auto with zarith. Qed. 
 
 
-    Lemma eval_SOS_red_add: forall n1 n2 (v1 : T n1) (v2 : T n2), (n2 <= n1)%nat -> small v1 -> small v2 -> eval (SOS_red_add v1 v2) = eval v1 + eval v2.
+  Lemma add_q_low_word: forall n (A : T (S n)), small A -> (eval A + eval (q n A k)) mod r = 0.
+  Proof.
+    intros. unfold q. rewrite eval_scmul; auto; try lia. unfold thism. Search (Z.mul_split).
+    rewrite Z.mul_split_mod. rewrite small_s_mod. rewrite Z.add_mod.
+    rewrite Z.mul_mod. repeat rewrite Z.mod_mod. rewrite <- Z.mul_mod.
+    rewrite <- Z.mul_assoc. rewrite Z.mul_mod. rewrite k_correct.
+    rewrite <- Z.mul_mod. Search (_ * (-1)). rewrite <- Z.opp_eq_mul_m1.
+    Search (_ + (- _)).
+    rewrite <- Z.add_mod. rewrite Z.add_opp_r.
+    rewrite Zminus_mod. rewrite Z.mod_mod. rewrite <- Zminus_mod.
+    Search (_ - _ = 0). rewrite Z.sub_diag. all: try unfold r; auto with zarith.
+    pose proof (smallthism' n A). unfold sc_small in H0. auto.
+  Qed.
+
+
+
+  Lemma r_nz: r <> 0.
+  Proof.
+    unfold r. auto with zarith.
+  Qed.
+
+    Lemma small_carry: forall n1 n2 (v1 : T n1) (v2 : T n2), (n2 <= n1)%nat -> small v1 -> small v2 ->
+    ((eval v1 + eval v2) / weight n1) <= 1.
     Proof.
-    Admitted.
+      intros. apply Z.div_floor; auto. simpl.  apply small_bound in H0. apply small_bound in H1.
+      pose proof (weight_geq' n1 n2 H). lia.
+    Qed.
+
+    Check S1.
+    Check s.
+
+    Lemma S1_mod_r: forall n (A : T (S n)), (R_numlimbs <= n)%nat -> small A -> eval (S1 n A k) mod r = 0.
+    Proof. intros n A H'' H'.
+      unfold S1. rewrite eval_SOS_add_full'; auto; try lia. Set Printing All. Search ((_ - _) mod _).
+      rewrite Zminus_mod. rewrite weight_value. Search (r ^ _). rewrite r_pow_S.
+      rewrite Z.mul_comm.
+      rewrite Z.mul_assoc. rewrite Z.mod_mul. simpl. Search (_ - 0). rewrite Z.sub_0_r.
+      rewrite Z.mod_mod. unfold q. unfold thism. rewrite eval_scmul. Search (fst (Z.mul_split _ _ _)).
+      rewrite Z.mul_split_mod. rewrite Z.add_mod. rewrite Z.mul_mod. rewrite Z.mod_mod.
+      rewrite (Z.mul_mod _ k _). rewrite <- Z.mul_mod. rewrite <- Z.mul_assoc. rewrite Z.mul_mod.
+      rewrite (Z.mul_mod _ (eval N) _). repeat rewrite Z.mod_mod.
+      rewrite <- (Z.mul_mod k _ _). rewrite k_correct.
+      rewrite <- Z.mul_mod. rewrite <- Z.add_mod. Search (_ * (-1)).
+      rewrite <- Z.opp_eq_mul_m1. rewrite Z.add_opp_r. Set Printing All.
+      
+      rewrite small_s_mod. Set Printing All.
+      rewrite Zminus_mod. rewrite Z.mod_mod. Search (?n1 - ?n1).
+      rewrite <- Zminus_mod. rewrite Z.sub_diag. all: (try apply r_nz; auto with zarith).
+      Search (fst (Z.mul_split _ _ _)). rewrite Z.mul_split_mod.
+      apply Z_mod_lt. unfold r; auto with zarith.
+      unfold q. apply small_scmul; auto. apply smallthism'.
+      lia.
+    Qed.
+
+    (* Lemma eval_SOS_red_add_mod: forall n1 n2 (v1 : T n1) (v2 : T n2), (n2 <= n1)%nat -> small v1 -> small v2 -> eval (SOS_red_add v1 v2) = (eval v1 + eval v2) mod r ^ Z.of_nat n1.
+    Proof.
+      intros. unfold SOS_red_add. simpl. unfold eval. rewrite Rows.sum_rows_mod; auto.
+        - rewrite weight_value. rewrite <- eval_extend with (n1 := n1); try apply length_small; auto.
+        - apply length_small; auto.
+        - rewrite extend_length; try apply length_small; auto.
+    Qed. *)
+
+
+    (* Lemma eval_SOS_red_add: forall n1 n2 (v1 : T n1) (v2 : T n2), (n2 <= n1)%nat -> small v1 -> small v2 -> eval (SOS_red_add v1 v2) = eval v1 + eval v2.
+    Proof.
+      intros. assert (small (SOS_red_add v1 v2)) by (apply small_SOS_red_add; auto). unfold SOS_red_add. unfold SOS_red_add in H2.
+      remember (Rows.add weight n1 v1 (Positional.extend_to_length n2 n1 v2)) as v'.
+      destruct v'. apply (f_equal (fun y => fst y)) in Heqv'. rewrite Rows.add_partitions in Heqv'; auto.
+      simpl in Heqv'. unfold small in H2. 
+    Admitted. *)
     
     Local Opaque T addT drop_high_addT' divmod zero scmul conditional_sub sub_then_maybe_add.
     Create HintDb push_mont_eval discriminated.
@@ -590,6 +846,95 @@ End red_loop.
 End mul_iteration_proofs.
 
 Section red_body_proofs.
+    Context (pred_A_numlimbs : nat)
+        (N_numlimbs : nat)
+        (A : T (S pred_A_numlimbs))
+        (small_A : @small (S pred_A_numlimbs) A)
+        (A_len : length A = S pred_A_numlimbs)
+        (A_big : (R_numlimbs <= pred_A_numlimbs)%nat)
+        (N_len : length N = R_numlimbs)
+        (N_eval: 0 <= eval N < r ^ Z.of_nat R_numlimbs).
+
+        Local Notation red_steps A := (@red_steps pred_A_numlimbs A k).
+
+        Lemma A_bounds: 0 <= eval A.
+        Proof.
+          apply small_bound; auto.
+        Qed.
+
+        Lemma q_bounds: 0 <= eval (q (pred_A_numlimbs) A k).
+        Proof.
+          apply small_bound; unfold q; apply small_scmul; auto; unfold thism; rewrite Z.mul_split_mod; auto with zarith.
+        Qed.
+        
+        Lemma smallthism: sc_small (thism pred_A_numlimbs A k).
+        Proof. clear small_A A_len; unfold thism; rewrite Z.mul_split_mod; unfold sc_small; auto with zarith. Qed. 
+
+        Lemma smallq: small (q pred_A_numlimbs A k).
+        Proof. unfold q; apply small_scmul; auto; apply smallthism. Qed.
+        Lemma smallS1 : small (S1 pred_A_numlimbs A k).
+        Proof. clear A_len; apply small_SOS_red_add; auto with zarith; apply small_scmul; auto; apply smallthism. Qed.
+
+        Lemma div_monot: forall a b c, 0 <= c -> a <= b -> a / c <= b / c.
+        Proof.
+          intros. apply Z.div_le_mono_nonneg; auto.
+        Qed. 
+
+        Local Open Scope Z_scope.
+        Lemma div_bound_aux: forall a b d, 0 < d -> b < d -> (a + b)/ d <= a / d + 1.
+        Proof. clear A_len A_big small_A.
+          intros. assert (a + b <= a + d) by lia; apply div_monot with (c := d) in H1; auto; try lia.
+          assert (a + d = a + d * 1) by auto with zarith; rewrite H2 in H1; rewrite Z.div_add' in H1; auto with zarith.
+        Qed.
+
+Lemma red_body_bounds: (S R_numlimbs < pred_A_numlimbs)%nat ->  (eval (red_steps A)) / (weight (Nat.pred pred_A_numlimbs)) <= (eval A) / (weight (pred_A_numlimbs)) + 1.
+Proof. pose proof smallq as Hq. intros H''.
+  destruct pred_A_numlimbs eqn:eq'; auto with zarith.
+  rewrite red_steps'. unfold S2. rewrite eval_div; try apply smallS1.
+  rewrite Zdiv_Zdiv; try lia; simpl.
+  pose proof (weight_value (S n)). rewrite Nat2Z.inj_succ in H. rewrite Z.pow_succ_r in H.
+  rewrite H. rewrite weight_value. simpl.
+  unfold S1. rewrite eval_SOS_add_full'; auto with zarith.
+  destruct (eval A + eval (q (S n) A k) <? (weight (S (S n)))) eqn:eq1.
+    - apply Z.ltb_lt in eq1. rewrite (Zdiv_small _ (weight _)).
+      + rewrite Z.mul_0_r. rewrite Z.sub_0_r. rewrite weight_value in eq1. rewrite Nat2Z.inj_succ in eq1.
+        rewrite Z.pow_succ_r in eq1; try lia.
+        apply div_bound_aux.
+        apply Z.mul_pos_pos. lia. unfold r. rewrite <- Z.pow_mul_r; auto with zarith.
+        apply small_bound in Hq. rewrite weight_value in Hq. rewrite Nat2Z.inj_succ in Hq. rewrite Z.pow_succ_r in Hq; try lia.
+        apply lt_S_n in H''.
+        assert (r * r ^ (Z.of_nat R_numlimbs) <= r * r ^ (Z.of_nat n)).
+        apply Z.mul_le_mono_pos_l; try lia. apply Zpow_facts.Zpower_le_monotone; try lia.
+        lia.
+      + split; auto. 
+        assert (small (q (S n) A k)) by (unfold q; apply small_scmul; auto; unfold thism; rewrite Z.mul_split_mod; auto with zarith).
+        apply Z.add_nonneg_nonneg; (apply small_bound; auto).
+    - Search (_ <? _ = false). apply Z.ltb_nlt in eq1. Search (?n1 <= ?n2).
+      assert (((eval A + eval (q (S n) A k)) / weight (S (S n))) = 1).
+        + apply Z.le_antisymm.
+          * apply small_carry; auto; lia.
+          * Search (0 < (_ / _)). Search ((_ + 1) <= _). assert (1 = 0 + 1) by auto. rewrite H0.
+            apply Ztac.Zlt_le_add_1. apply Z.div_str_pos. Search (~ (_ < _)). apply Z.nlt_ge in eq1.
+            split; try lia. apply wprops.
+        + rewrite H0. pose proof (small_bound Hq). rewrite Z.add_1_r.
+          Search ( _ <= Z.succ _). apply Z.le_succ_r; left. apply div_monot; try lia.
+          apply Z.mul_nonneg_nonneg; try apply Z.pow_nonneg; lia.
+          rewrite Z.mul_1_r. assert (weight (S R_numlimbs) <= weight (S (S n))). apply weight_geq'; lia.
+          lia.
+    - lia.
+    - pose proof wprops as Hw; destruct Hw. pose proof (weight_positive n); lia.
+    - unfold S1. apply small_SOS_red_add; auto; try lia.
+Qed.
+
+(* Lemma red_body_bounds_final. (S R_numlimbs = pred_A_numlimbs)%nat ->  (eval (red_steps A)) / (weight (Nat.pred pred_A_numlimbs)) <= (eval A) / (weight (pred_A_numlimbs)) + 1.
+           *)
+
+
+
+End red_body_proofs.
+
+
+Section red_body_proofs.
       Context (pred_A_numlimbs : nat)
               (N_numlimbs : nat)
               (A : T (S pred_A_numlimbs))
@@ -622,12 +967,23 @@ Section red_body_proofs.
       - auto.
   Qed.
 
-  Lemma eval_red_body: eval (red_body A) = (eval A + (eval N) * ((s * k) mod r)) / r.
+   (* Lemma eval_red_body_mod: r * eval (red_body A) mod eval N = (eval A) mod eval N.
+  Proof.
+    unfold red_body. rewrite red_steps'. unfold S2.
+    rewrite eval_div. Search (?n1 * (_ / ?n1)). rewrite Z.mul_div_eq_full.
+    rewrite S1_mod_r. rewrite Z.sub_0_r.
+    unfold S1. rewrite eval_SOS_add_full'.
+
+    apply (f_equal (fun (y : Z) => (y / r) mod eval N)).
+    unfold S1.  *)
+
+
+  (* Lemma eval_red_body: eval (red_body A) = (eval A + (eval N) * ((s * k) mod r)) / r.
   Proof.
     unfold red_body. rewrite red_steps'. unfold S2.
     rewrite eval_div. apply (f_equal (fun (y : Z) => (y / r))).
     unfold S1.
-    rewrite eval_SOS_red_add. apply (f_equal (fun y => eval A + y)). unfold q.
+    rewrite eval_SOS_red_add.  apply (f_equal (fun y => eval A + y)). unfold q.
     rewrite eval_scmul. rewrite Z.mul_comm. apply (f_equal (fun y => eval N * y)).
     unfold thism. rewrite Z.mul_split_mod.
     all: auto.
@@ -636,13 +992,13 @@ Section red_body_proofs.
       - unfold q. apply small_scmul; auto. unfold thism. rewrite Z.mul_split_mod. apply Z_mod_lt. lia.
       - unfold S1. apply small_SOS_red_add; auto; try lia. unfold q. apply small_scmul; auto.
         unfold thism. rewrite Z.mul_split_mod. apply Z_mod_lt. lia.
-  Qed.
+  Qed. *)
 
   Lemma divmod_A: eval A mod r = s.
     unfold s, A_s. rewrite eval_mod. auto. auto.
   Qed.
 
-  Lemma eval_red_body_mul_r: r * eval (red_body A) = (eval A + (eval N) * ((s * k) mod r)).
+  (* Lemma eval_red_body_mul_r: r * eval (red_body A) = (eval A + (eval N) * ((s * k) mod r)).
   Proof.
     rewrite eval_red_body. Search ((_ / _) * _). rewrite Z.mul_div_eq.
     assert ((eval A + eval N * ((s * k) mod r)) mod r = 0).
@@ -654,7 +1010,7 @@ Section red_body_proofs.
         Search (_ + ( - _)). rewrite Z.add_opp_diag_r. auto with zarith.
       - rewrite H. auto with zarith.
       - lia. 
-  Qed.
+  Qed. *)
 
   Lemma div_nil: forall n, @divmod n [] = ([], 0).
   Proof. reflexivity. Qed.
@@ -712,8 +1068,8 @@ Check first_n.
     intros. rewrite red_loop_comm. auto.
   Qed.
 
-  Lemma small_red_loop: forall init count A, small A -> (R_numlimbs <= init)%nat -> (length (A) = init + count + 1)%nat -> small (red_loop (init) count A).
-  Proof.
+  Lemma small_red_loop: forall init count (A : T (init + count + 1)), small A -> (R_numlimbs <= init)%nat -> (length (A) = init + count + 1)%nat -> small (red_loop (init) count A).
+  Proof. clear A_big.
     intros. generalize dependent init. induction count.
       - intros. unfold red_loop. simpl. Set Printing All. rewrite Nat.add_0_r in H. auto.
       - intros. rewrite red_loop_next. apply (IHcount). apply small_red_body.
@@ -729,15 +1085,388 @@ Check first_n.
   Qed.
 
   Lemma length_red_loop: forall init count A, (R_numlimbs <= init)%nat -> (length A = init + count + 1)%nat -> length (red_loop init count A) = (init + 1)%nat.
-  Proof. intros. generalize dependent A. generalize dependent init. induction count.
+  Proof. clear A_big. intros. generalize dependent A. generalize dependent init. induction count.
     - intros. unfold red_loop. simpl. auto with zarith.
     - intros. rewrite red_loop_next'. rewrite length_red_body; auto with zarith.
       + rewrite (IHcount (S init)). auto. auto with zarith. lia.
       + rewrite <- Nat.add_succ_comm. lia.
   Qed. 
 
-  Check red_body.
-  Lemma eval_red_loop: forall init count (A : T (init + count + 1)), (length A = init + count + 1)%nat -> (R_numlimbs <= init)%nat -> small A -> (eval A) mod eval N = (r ^Z.of_nat count * eval (red_loop init count A)) mod eval N.
+  End red_loop_proofs.
+
+  Section red_loop_proofs'.
+  Context (pred_A_numlimbs : nat)
+          (N_numlimbs : nat)
+          (N_len : length N = R_numlimbs)
+          (A_big : (R_numlimbs <= pred_A_numlimbs)%nat)
+          (N_eval: 0 <= eval N < r ^ Z.of_nat R_numlimbs)
+          (A : T (R_numlimbs + R_numlimbs))
+          (A_bound : eval A < eval N * eval N)
+          (A' : T (S (R_numlimbs + R_numlimbs)) := Positional.extend_to_length (R_numlimbs + R_numlimbs) (S (R_numlimbs + R_numlimbs)) A)
+          (A_small: small A).
+
+  Definition A_it (iterations : nat) := red_loop (R_numlimbs + R_numlimbs - iterations) k iterations A'.        
+
+Check A_it.
+
+  Lemma small_A': small A'.
+  Proof. unfold A'. apply small_exten; auto. Qed.
+
+  Lemma small_A_it : forall it, (it <= R_numlimbs)%nat -> small (A_it it).
+  Proof.
+    intros. unfold A_it. apply small_red_loop. all: (auto with zarith; try lia).
+    Search Positional.extend_to_length. assert (S (R_numlimbs + R_numlimbs) = (R_numlimbs + R_numlimbs - it + it + 1)%nat). auto with zarith.
+    rewrite <- H0. apply small_exten. lia. auto.
+    apply length_small in A_small. unfold A'. rewrite extend_length; auto with zarith.
+  Qed.
+
+  (* Lemma red_loop_bound_N: forall it, (0 < it <= R_numlimbs)%nat ->
+  eval (A_it it) < eval N * r ^ (Z.of_nat (R_numlimbs - it)) + eval N.
+  Proof.
+    intros. destruct it; try (exfalso; apply (Nat.lt_irrefl O); lia).
+    induction it.
+      - unfold A_it. simpl. unfold red_body. rewrite red_steps'.
+        unfold S2. rewrite Nat.add_0_r. assert (forall y, 0 < y -> y + y -1 + 1 = y + y)%nat by auto with zarith.
+        rewrite H0; try lia. rewrite eval_div. Search ( (_ * ?n1) / ?n1). Search (_ < _).
+        assert (forall y, y = Z.succ (y - 1)) by auto with zarith.
+        rewrite (H1 (_ + eval N)).
+        apply Zle_lt_succ.
+        rewrite <- (Z_div_mult (_ -1) r). Search ( (_ / ?n1) <= (_ / ?n1)).
+        apply div_monot; try lia. unfold S1.
+        assert (eval (SOS_red_add A' (q (R_numlimbs + R_numlimbs) A' k)) <= eval A' + eval (q (R_numlimbs + R_numlimbs) A' k)).
+        {
+          apply eval_SOS_bound; try lia; try apply small_A'. unfold q.
+          apply small_scmul; auto; apply smallthism'.
+        }
+        rewrite Z.mul_sub_distr_r. rewrite Z.mul_1_l.
+        rewrite Z.mul_add_distr_r.
+        rewrite <- Z.mul_assoc. rewrite (Z.mul_comm _ r).
+        rewrite <- Z.pow_succ_r. rewrite <- Nat2Z.inj_succ.
+        assert (S (R_numlimbs - 1) = R_numlimbs) by auto with zarith. rewrite H2.
+        assert (eval A' < eval N * r ^ Z.of_nat R_numlimbs - r).
+        {
+          unfold A'. rewrite <- eval_extend. pose proof (small_bound A_small).
+          pose proof (small_bound small_N). destruct H5. rewrite (H1 (weight _)) in H6.
+          apply Z.lt_succ_r in H6. assert (eval N * eval N <= (weight R_numlimbs - 1) * (weight R_numlimbs - 1)).
+          Search (_ * _ <= _ * _). apply Z.mul_le_mono_nonneg; auto; try lia.
+          rewrite Z.mul_sub_distr_l in H7. repeat rewrite Z.mul_sub_distr_r in H7.
+          repeat rewrite Z.mul_1_r in H7. rewrite Z.mul_1_l in H7. Search (_ - (_ - _)).
+          rewrite Z.sub_sub_distr in H7. Search (_ - _ = 0).
+          assert (forall y, y + 1 = Z.succ y) by auto.
+          assert (weight R_numlimbs * weight R_numlimbs - weight R_numlimbs -
+          weight R_numlimbs + 1 <)
+          
+          rewrite H8 in H7.
+          apply Z.lt_succ_r in H7.
+          
+          
+          
+          rewrite weight_value in H4.
+          assert (eval N * eval N < eval N * r ^ Z.of_nat R_numlimbs) by (apply Zmult_gt_0_lt_compat_l; try lia).
+          lia. lia. apply length_small; auto.
+        }
+        assert (eval (q (R_numlimbs + R_numlimbs) A' k) < eval N * r).
+        {
+          unfold q. rewrite eval_scmul. pose proof (smallthism' (R_numlimbs + R_numlimbs) A').
+          unfold sc_small in H4. rewrite Z.mul_comm. apply Zmult_gt_0_lt_compat_l; try lia.
+          all: auto. apply smallthism'.
+        }
+        lia. lia. lia.
+        unfold S1. apply small_SOS_red_add; try lia. apply small_A'. unfold q. apply small_scmul; auto. apply smallthism'.
+      - remember (S it) as it'. unfold A_it in IHit.
+        assert (HZ: (R_numlimbs + R_numlimbs - it' + it' + 1)%nat = (S (R_numlimbs + R_numlimbs))%nat) by auto with zarith.
+        assert (S (R_numlimbs + R_numlimbs - (S it')) = R_numlimbs + R_numlimbs - it')%nat by auto with zarith.
+        unfold A_it. rewrite red_loop_next'. repeat rewrite Nat.add_1_r. unfold red_body.
+        rewrite red_steps'. unfold S2. rewrite eval_div. rewrite H0. unfold S1.
+
+        assert ( eval
+        (SOS_red_add (red_loop (R_numlimbs + R_numlimbs - it') k it' A')
+           (q (R_numlimbs + R_numlimbs - it')
+              (red_loop (R_numlimbs + R_numlimbs - it') k it' A') k)) 
+          <= eval (red_loop (R_numlimbs + R_numlimbs - it') k it' A') + eval (q (R_numlimbs + R_numlimbs - it')
+          (red_loop (R_numlimbs + R_numlimbs - it') k it' A') k)).
+          apply eval_SOS_bound; try lia.
+          + apply small_red_loop; try lia. rewrite HZ. apply small_A'.
+            rewrite HZ. apply length_small. apply small_A'.
+          + unfold q; apply small_scmul; auto; apply smallthism'.
+          + rewrite <- (Z_div_mult (_ + eval N) r).
+            (* apply div_monot; try lia. *)
+            rewrite Z.mul_add_distr_r. rewrite <- Z.mul_assoc.
+            assert (r ^ Z.of_nat (R_numlimbs - S it') * r = r ^ Z.of_nat (R_numlimbs - it')).
+            {
+              rewrite Z.mul_comm. rewrite <- Z.pow_succ_r. rewrite <- Nat2Z.inj_succ.
+              assert (S (R_numlimbs - S it') = R_numlimbs - it')%nat by auto with zarith.
+              rewrite H2. auto. lia.
+            }
+            rewrite H2.
+            assert (0 < it' <= R_numlimbs)%nat by lia.
+            remember (IHit H3) as H4. destruct HeqH4.
+            Search ( (_ + _ * ?n1) / ?n1). rewrite Z_div_plus_full; auto with zarith.
+
+            apply (div_monot _ _ r) in H4.
+            assert (R_numlimbs - it' = 1)%nat. rewrite by auto with zarith.
+            
+            assert (eval (red_loop (R_numlimbs + R_numlimbs - it') k it' A') < eval N * r ^ (Z.of_nat (R_numlimbs - it'))).
+          
+          assert (eval)
+        
+        assert (eval (S1 (R_numlimbs + R_numlimbs) A' k) < eval N * r ^ (Z.of_nat))
+        
+        
+        pose proof (eval_div R_numlimbs + R_numlimbs).
+        Set Printing All. rewrite Nat.add_1_r.
+        Set Printing All. repeat rewrite Nat.sub_0_r. rewrite <- H0.
+ *)
+
+  Lemma red_loop_it: forall it, (it < R_numlimbs)%nat -> eval (A_it it) / weight (R_numlimbs + R_numlimbs - it) <= Z.of_nat it.
+  Proof.
+    intros it H'. induction it.
+      - unfold A_it. unfold red_loop. simpl. assert (small A') by (apply small_exten; auto; try lia).
+        Search (_ / _ = 0). rewrite Zdiv_small; auto with zarith. unfold A'.
+        rewrite Nat.sub_0_r. rewrite Nat.add_1_r.
+        rewrite <- eval_extend. apply small_bound in A_small. auto. lia.
+        apply length_small in A_small. auto.
+      - unfold A_it. unfold A_it in IHit. rewrite red_loop_next'.
+        assert (S (R_numlimbs + R_numlimbs - S it) = R_numlimbs + R_numlimbs - it)%nat by auto with zarith.
+        rewrite H.
+        remember (red_loop (R_numlimbs + R_numlimbs - it) k it A') as A''.
+        assert (eval (red_body k (red_loop (S (R_numlimbs + R_numlimbs - S it)) k it A')) /
+        weight (R_numlimbs + R_numlimbs - S it) <= eval A'' / weight (R_numlimbs + R_numlimbs - it) + 1).
+          {
+             rewrite H. rewrite <- HeqA''. Check red_body. unfold red_body.
+             pose proof (red_body_bounds (R_numlimbs + R_numlimbs - it) A'').
+             rewrite Nat.add_1_r. assert (R_numlimbs + R_numlimbs - S it = Nat.pred (R_numlimbs + R_numlimbs - it))%nat by auto with zarith.
+             rewrite H1. Search (S (Nat.pred _)). rewrite NPeano.Nat.succ_pred_pos; try lia.
+             rewrite Nat.add_1_r. apply H0. pose proof (length_small small_N).
+             rewrite HeqA''. assert (0 <= eval N < r ^ Z.of_nat R_numlimbs) by auto.
+             pose proof (small_red_loop H2 H3 (R_numlimbs + R_numlimbs - it) it A').
+            repeat rewrite Nat.add_1_r in H4. apply H4. assert (S (R_numlimbs + R_numlimbs - it + it) = S (R_numlimbs + R_numlimbs)). auto with zarith.
+            rewrite H5. apply small_A'.
+            all: auto with zarith; try lia.
+            unfold A'. Search Positional.extend_to_length. rewrite extend_length; auto with zarith; try lia.
+            pose proof (length_small A_small). auto.
+            rewrite HeqA''. pose proof (length_small small_N).
+            pose proof (length_red_loop H2 (R_numlimbs + R_numlimbs - it) it A').
+            repeat rewrite Nat.add_1_r in H3. apply H3; try lia.
+            unfold A'. assert (S (R_numlimbs + R_numlimbs - it + it) = S (R_numlimbs + R_numlimbs)) by auto with zarith.
+            rewrite H4. apply extend_length; auto; try lia. apply length_small; auto. 
+          }
+        assert (S (R_numlimbs + R_numlimbs - S it)= R_numlimbs + R_numlimbs - it)%nat by auto with zarith.
+        rewrite H1 in H0. rewrite <- HeqA'' in H0.
+        repeat rewrite Nat.add_1_r. repeat rewrite Nat.add_1_r in H0.
+        repeat rewrite Nat.add_1_r in IHit. assert (it < R_numlimbs)%nat by lia.
+        apply IHit in H2. lia.
+  Qed.
+
+  Lemma add_small_it: forall it, (it < R_numlimbs)%nat -> eval (A_it it) + eval (q (R_numlimbs + R_numlimbs - it) (A_it it) k)
+    < weight (S (R_numlimbs + R_numlimbs - it)).
+  Proof. intros. (*remove these pose proofs*) pose proof Z.add_0_r. pose proof Z.add_0_l. 
+    pose proof (red_loop_it it). assert (it < R_numlimbs)%nat by lia.
+    apply H2 in H3.
+    Search (_ * ?n1 <= _ * ?n1). apply (Z.mul_le_mono_pos_r _ _ (weight (R_numlimbs + R_numlimbs - it))) in H3.
+    Search (_ / _). rewrite Z.mul_comm in H3. rewrite Z.mul_div_eq_full in H3.
+    Search (_ + ?n1 <= _ + ?n1).
+    apply (Z.add_le_mono_r _ _ (eval (A_it it) mod weight (R_numlimbs + R_numlimbs - it))) in H3.
+    simpl in H3. Search (_ - ?n1 + ?n1 = _). rewrite Z.sub_add in H3.
+    assert (eval (A_it it) mod weight (R_numlimbs + R_numlimbs - it) < weight (R_numlimbs + R_numlimbs - it)). Search (_ mod _ < _).
+    apply Z.mod_bound_pos. apply small_bound. rewrite Nat.add_1_r. auto.
+    unfold A_it. pose proof (length_small small_N) as HN.
+    pose proof (small_bound small_N) as HN'. rewrite weight_value in HN'.
+    pose proof (small_red_loop HN HN' (R_numlimbs + R_numlimbs - it) it A').
+    repeat rewrite Nat.add_1_r in H4. apply H4. pose proof small_A'.
+    assert (R_numlimbs + R_numlimbs - it + it = R_numlimbs + R_numlimbs)%nat by auto with zarith.
+    rewrite H6. auto. lia.
+    assert (R_numlimbs + R_numlimbs - it + it = R_numlimbs + R_numlimbs)%nat by auto with zarith.
+    rewrite H5. apply length_small. apply small_A'. auto with zarith.
+    assert ( (Z.of_nat it) * weight (R_numlimbs + R_numlimbs - it) + eval (A_it it) mod weight (R_numlimbs + R_numlimbs - it) < (Z.of_nat it + 1) * weight (R_numlimbs + R_numlimbs - it)) by lia.
+    assert (eval (A_it it) <=  (Z.of_nat it + 1) * weight (R_numlimbs + R_numlimbs - it)) by lia.
+    assert (small (q (R_numlimbs + R_numlimbs - it)
+    (red_loop (R_numlimbs + R_numlimbs - it) k it A') k)).
+      * unfold q. apply small_scmul; auto; apply smallthism'.
+      * apply small_bound in H7.
+      assert (weight (S R_numlimbs) + (Z.of_nat it + 1) * weight (R_numlimbs + R_numlimbs - it) <= weight (S (R_numlimbs + R_numlimbs - it))).
+      {
+        repeat rewrite weight_value.
+        assert (Z.of_nat it + 1 <= r - 1). lia. 
+        assert ((Z.of_nat it + 1) * r ^ Z.of_nat (R_numlimbs + R_numlimbs - it) <= (r - 1) * r ^ Z.of_nat ((R_numlimbs + R_numlimbs - it))).
+        Search ( (_ + _) * _).
+        Search ( _ * _ <= _ * _).
+        Set Printing All. apply Z.mul_le_mono_nonneg_r. assert (O < R_numlimbs + R_numlimbs - it)%nat by lia.
+        unfold r. Search (0 <= _ ^ _). Search ((_ ^ _) ^ _). rewrite <- Z.pow_mul_r.
+        apply Pow2.Z.pow2_ge_0. all: try lia.
+        assert (r ^ Z.of_nat (S R_numlimbs) <= r ^ Z.of_nat (R_numlimbs + R_numlimbs - it)).
+        Search (_ ^ _ <= _). pose proof (Z.pow_le_mono_r r (Z.of_nat (S R_numlimbs)) (Z.of_nat (R_numlimbs + R_numlimbs - it))).
+        apply H10. all: try lia.
+        rewrite Z.mul_sub_distr_r in H9. rewrite Z.mul_1_l in H9.
+        Search (_ + _ <= _ + _). 
+        rewrite (Z.add_le_mono_r _ _ (r ^ Z.of_nat (R_numlimbs + R_numlimbs - it))) in H9.
+        Search (_ - ?n1 + ?n1). rewrite Z.sub_add in H9.
+        rewrite Z.add_comm in H9. Search (_ ^ (Z.succ _)). rewrite (Nat2Z.inj_succ (R_numlimbs + R_numlimbs - it) ).
+        rewrite (Z.pow_succ_r  _ (Z.of_nat (R_numlimbs + R_numlimbs - it))). lia.
+        lia.
+      }
+      unfold A_it in H6. rewrite Z.add_comm in H8.
+      assert ( (eval (red_loop (R_numlimbs + R_numlimbs - it) k it A') +
+      eval
+        (q (R_numlimbs + R_numlimbs - it)
+           (red_loop (R_numlimbs + R_numlimbs - it) k it A') k)) < (Z.of_nat it + 1) * weight (R_numlimbs + R_numlimbs - it) +
+           weight (S R_numlimbs)). lia. repeat rewrite Nat.add_1_r in H9. unfold A_it.
+           lia.
+      * auto.
+      * rewrite weight_value. unfold r. rewrite <- Z.pow_mul_r.
+        Search (0 < _ ^ _). apply Pow2.Z.pow2_gt_0. assert (0 < R_numlimbs + R_numlimbs - it)%nat by lia.
+        lia. lia. lia.
+  Qed.
+
+  Lemma red_loop_it_mod: forall it, (it < R_numlimbs)%nat -> ((r ^ Z.of_nat it * eval (A_it it) mod eval N)
+    = eval A mod eval N).
+  Proof.
+    intros. assert (Haux: (R_numlimbs + R_numlimbs - it + it)%nat = (R_numlimbs + R_numlimbs)%nat) by auto with zarith.
+    assert (small_A_it: small (A_it it)). unfold A_it. apply small_red_loop; auto. 
+    rewrite Haux. rewrite Nat.add_1_r. apply small_A'. lia. rewrite Haux. rewrite Nat.add_1_r. apply length_small. apply small_A'. 
+     induction it.
+      - unfold A_it. unfold red_loop. simpl. Set Printing All. simpl. assert (eval A = eval A'). unfold A'. rewrite <- eval_extend. auto.
+      auto. apply length_small. auto. rewrite Nat.sub_0_r. rewrite Nat.add_1_r.
+      rewrite H0. 
+      Set Printing All.
+      
+      auto.
+      destruct (eval A'); auto.
+      - unfold A_it. rewrite red_loop_next'. rewrite r_pow_S.
+        assert (it < R_numlimbs)%nat by lia. apply IHit in H0.
+         repeat rewrite Nat.add_1_r. unfold red_body. rewrite red_steps'.
+         unfold S2. Search (eval (fst (divmod _))). rewrite eval_div.
+         rewrite <- Z.mul_assoc. Search (?n1 * (_ / ?n1)).
+         rewrite Z.mul_div_eq_full. rewrite S1_mod_r. rewrite Z.sub_0_r.
+         unfold A_it in H0. unfold S1. rewrite eval_SOS_add_small.
+         unfold q. rewrite eval_scmul. rewrite Z.mul_mod. rewrite Z.add_mod.
+         Search ( (_ * ?n1 mod ?n1)). rewrite Z.mod_mul. rewrite Z.add_0_r.
+         rewrite <- Z.mod_mod. rewrite <- Z.mul_mod. rewrite Z.mod_mod.
+         assert (S (R_numlimbs + R_numlimbs - S it) = (R_numlimbs + R_numlimbs - it))%nat by auto with zarith.
+         rewrite H1. 
+         Set Printing All. rewrite Nat.add_1_r in H0.
+         rewrite Z.mul_mod. rewrite Z.mod_mod. rewrite <- Z.mul_mod. auto.
+         all: auto; try lia.
+          + apply smallthism'.
+          + pose proof (length_small small_N) as HN.
+            pose proof (small_bound small_N) as HN'. rewrite weight_value in HN'.
+           pose proof (small_red_loop HN HN' (R_numlimbs + R_numlimbs - it) it A').
+          assert (S (R_numlimbs + R_numlimbs - S it) = (R_numlimbs + R_numlimbs - it))%nat by auto with zarith.
+          rewrite H2.
+           Set Printing All. repeat rewrite Nat.add_1_r in H1. apply H1.
+           assert (R_numlimbs + R_numlimbs - it + it = R_numlimbs + R_numlimbs)%nat by auto with zarith.
+           rewrite H3. apply small_A'. lia.
+           assert (R_numlimbs + R_numlimbs - it + it = R_numlimbs + R_numlimbs)%nat by auto with zarith.
+           rewrite H3. apply length_small. apply small_A'.
+          + unfold q. apply small_scmul; auto; try lia. apply smallthism'.
+          + assert (S (R_numlimbs + R_numlimbs - S it) = (R_numlimbs + R_numlimbs - it))%nat by auto with zarith.
+            rewrite H1. pose proof (add_small_it it). unfold A_it in H2.
+            rewrite Nat.add_1_r in H2. apply H2. lia.
+          + assert (HN: length N = R_numlimbs). apply length_small; auto.
+            pose proof (small_bound small_N) as HN'. rewrite weight_value in HN'.
+            pose proof (small_red_loop HN HN' ( (R_numlimbs + R_numlimbs - it)) it). Set Printing All.
+            assert ((S (Init.Nat.sub (Init.Nat.add R_numlimbs R_numlimbs) (S it)) =  (Init.Nat.sub (Init.Nat.add R_numlimbs R_numlimbs) ( it)))) by auto with zarith.
+            rewrite H2. repeat rewrite Nat.add_1_r in H1.
+            Set Printing All.
+            apply H1.
+            assert (R_numlimbs + R_numlimbs - it + it = R_numlimbs + R_numlimbs)%nat by auto with zarith.
+            rewrite H3. apply small_A'. lia.
+            assert (R_numlimbs + R_numlimbs - it + it = R_numlimbs + R_numlimbs)%nat by auto with zarith.
+            rewrite H3. apply extend_length; auto. apply length_small. auto.
+          + unfold S1. apply small_SOS_red_add; try lia.
+            assert (HN: length N = R_numlimbs). apply length_small; auto.
+            pose proof (small_bound small_N) as HN'. rewrite weight_value in HN'.
+            pose proof (small_red_loop HN HN' ( (R_numlimbs + R_numlimbs - it)) it). Set Printing All.
+            assert ((S (Init.Nat.sub (Init.Nat.add R_numlimbs R_numlimbs) (S it)) =  (Init.Nat.sub (Init.Nat.add R_numlimbs R_numlimbs) ( it)))) by auto with zarith.
+            rewrite H2. repeat rewrite Nat.add_1_r in H1.
+            Set Printing All.
+            apply H1.
+            assert (R_numlimbs + R_numlimbs - it + it = R_numlimbs + R_numlimbs)%nat by auto with zarith.
+            rewrite H3. apply small_A'. lia.
+            assert (R_numlimbs + R_numlimbs - it + it = R_numlimbs + R_numlimbs)%nat by auto with zarith.
+            rewrite H3. apply extend_length; auto. apply length_small. auto.
+            unfold q. apply small_scmul; auto; apply smallthism'.
+          + Set Printing All. repeat rewrite Nat.add_1_r.
+            unfold A_it.
+            assert (HN: length N = R_numlimbs). apply length_small; auto.
+            pose proof (small_bound small_N) as HN'. rewrite weight_value in HN'.
+            pose proof (small_red_loop HN HN' ( (R_numlimbs + R_numlimbs - it)) it). Set Printing All.
+            assert ((S (Init.Nat.sub (Init.Nat.add R_numlimbs R_numlimbs) (S it)) =  (Init.Nat.sub (Init.Nat.add R_numlimbs R_numlimbs) ( it)))) by auto with zarith.
+            repeat rewrite Nat.add_1_r in H1.
+            Set Printing All.
+            apply H1.
+            assert (R_numlimbs + R_numlimbs - it + it = R_numlimbs + R_numlimbs)%nat by auto with zarith.
+            rewrite H3. apply small_A'. lia.
+            assert (R_numlimbs + R_numlimbs - it + it = R_numlimbs + R_numlimbs)%nat by auto with zarith.
+            rewrite H3. apply extend_length; auto. apply length_small. auto.
+  Qed.
+
+
+  Lemma red_loop_final: (r ^ Z.of_nat R_numlimbs) * eval (A_it R_numlimbs) mod eval N = eval A mod eval N.
+  Proof.
+    unfold A_it. assert (forall (y : nat), y + y - y = y)%nat by auto with zarith. rewrite H.
+    assert (exists x, R_numlimbs = S x). apply Nat.neq_0_r. auto. destruct H0.
+    assert (eval (red_loop R_numlimbs k R_numlimbs A') = eval (red_loop R_numlimbs k (S x) A')) by (rewrite <- H0; auto).
+    rewrite H1. rewrite red_loop_next'. repeat rewrite Nat.add_1_r. unfold red_body.
+    rewrite red_steps'. unfold S2. Search (eval (fst (divmod _))). rewrite eval_div.
+    unfold S1. rewrite eval_SOS_add_small. assert (r ^ Z.of_nat R_numlimbs = r ^ (Z.of_nat (S x))).
+    rewrite H0. auto.
+    rewrite H2. rewrite r_pow_S. rewrite <- Z.mul_assoc. Search (?n1 * (_ / ?n1)).
+    rewrite Z.mul_div_eq. Search (_ mod r). pose proof S1_mod_r. unfold S1 in H3.
+    unfold SOS_red_add in H3. rewrite add_q_low_word.
+    rewrite Z.sub_0_r. unfold q. rewrite eval_scmul. Search (_ * (_ + _)).
+    rewrite Z.mul_add_distr_l. rewrite Z.add_mod. Search ( _ * ?n1 mod ?n1).
+    rewrite Z.mul_assoc. rewrite Z_mod_mult. rewrite Z.add_0_r.
+    rewrite Z.mul_mod. rewrite Z.mod_mod. rewrite <- Z.mul_mod.
+    assert (x < R_numlimbs)%nat by lia.
+    pose proof (red_loop_it_mod x H4). unfold A_it in H5.
+    assert (R_numlimbs + R_numlimbs - x = S R_numlimbs)%nat. auto with zarith.
+    rewrite H6 in H5. rewrite Nat.add_1_r in H5. 
+    apply H5. all: auto with zarith; try lia.
+    - apply smallthism'.
+    - assert (HN: length N = R_numlimbs). apply length_small; auto.
+      pose proof (small_bound small_N) as HN'. rewrite weight_value in HN'.
+      pose proof (small_red_loop HN HN' (S R_numlimbs ) x A'). Set Printing All.
+      assert ((S (Init.Nat.sub (Init.Nat.add R_numlimbs R_numlimbs) (S x)) =  (Init.Nat.sub (Init.Nat.add R_numlimbs R_numlimbs) ( x)))) by auto with zarith.
+      repeat rewrite Nat.add_1_r in H4. Set Printing All.
+      apply H4. pose proof small_A'.
+      unfold small. unfold small in H6.
+      assert (R_numlimbs + R_numlimbs = S R_numlimbs + x)%nat by auto with zarith.
+      rewrite <- H7. auto. lia.
+      unfold A'. rewrite extend_length. auto with zarith.
+      apply length_small; auto. lia.
+    - assert (HN: length N = R_numlimbs). apply length_small; auto.
+      pose proof (small_bound small_N) as HN'. rewrite weight_value in HN'.
+      pose proof (small_red_loop HN HN' (S R_numlimbs ) x A'). Set Printing All.
+      assert ((S (Init.Nat.sub (Init.Nat.add R_numlimbs R_numlimbs) (S x)) =  (Init.Nat.sub (Init.Nat.add R_numlimbs R_numlimbs) ( x)))) by auto with zarith.
+      repeat rewrite Nat.add_1_r in H2. Set Printing All.
+      apply H2. pose proof small_A'.
+      unfold small. unfold small in H4.
+      assert (R_numlimbs + R_numlimbs = S R_numlimbs + x)%nat by auto with zarith.
+      rewrite <- H5. auto. lia.
+      unfold A'. rewrite extend_length. auto with zarith.
+      apply length_small; auto. lia.
+    - unfold q. apply small_scmul; auto; apply smallthism'.
+    - assert (S R_numlimbs = R_numlimbs + R_numlimbs - x)%nat by auto with zarith.
+      repeat rewrite H2. pose proof (add_small_it x). unfold A_it in H3. rewrite Nat.add_1_r in H3.
+      rewrite H2 in H3. apply H3. lia.
+    - unfold S1. apply small_SOS_red_add; try lia.
+      assert (HN: length N = R_numlimbs). apply length_small; auto.
+      pose proof (small_bound small_N) as HN'. rewrite weight_value in HN'.
+      pose proof (small_red_loop HN HN' (S R_numlimbs ) x A'). Set Printing All.
+      assert ((S (Init.Nat.sub (Init.Nat.add R_numlimbs R_numlimbs) (S x)) =  (Init.Nat.sub (Init.Nat.add R_numlimbs R_numlimbs) ( x)))) by auto with zarith.
+      repeat rewrite Nat.add_1_r in H2. Set Printing All.
+      apply H2. pose proof small_A'.
+      unfold small. unfold small in H4.
+      assert (R_numlimbs + R_numlimbs = S R_numlimbs + x)%nat by auto with zarith.
+      rewrite <- H5. auto. lia.
+      unfold A'. rewrite extend_length. auto with zarith.
+      apply length_small; auto. lia.
+      unfold q. apply small_scmul; auto; apply smallthism'.
+  Qed.
+
+
+  (* Lemma eval_red_loop: forall init count (A : T (init + count + 1)), (length A = init + count + 1)%nat -> (R_numlimbs <= init)%nat -> small A -> (eval A) mod eval N = (r ^Z.of_nat count * eval (red_loop init count A)) mod eval N.
   Proof. intros. generalize dependent A. generalize dependent init. induction count.
     - intros. simpl. auto with zarith. Set Printing All. rewrite Nat.add_0_r. auto.
       destruct (eval A) eqn:eq1.
@@ -771,9 +1500,18 @@ Check first_n.
         + auto.
         + auto.
         + lia.
-  Qed.
+  Qed. *)
+  
 
-    (* Recurse for a as many iterations as A has limbs, varying A := A, S := 0, r, bounds
+  (* Lemma eval_loop_full: forall (A : T (S (R_numlimbs + R_numlimbs))), small A -> length A = S (R_numlimbs + R_numlimbs) -> eval A mod eval N = (r ^ Z.of_nat R_numlimbs) * eval (red_loop R_numlimbs R_numlimbs A) mod eval N.
+  Proof. 
+    intros. rewrite <- eval_red_loop; repeat rewrite Nat.add_succ_comm; repeat rewrite Nat.add_1_r; auto.
+  Qed. *)
+
+
+
+
+  (* Recurse for a as many iterations as A has limbs, varying A := A, S := 0, r, bounds
     Section Iteration_proofs.
       Context (pred_A_numlimbs : nat)
               (A : T (S pred_A_numlimbs))
